\subsection{Composition of Linear Transformations, Matrix Multiplication}

\begin{proposition}
    Composition is associative; given $T : V \to W, S : W \to U,$ and $R : U \to X$, then \[
    (R \circ S) \circ T = R \circ (S \circ T).
    \]
\end{proposition}
\begin{proof}
    Fix $v \in V$. Then \begin{align*}
        (R \circ S) \circ T(v) = (R\circ S)(T(v)) = R (S(T(v)))
    \end{align*}
    OTOH:
    \begin{align*}
        R\circ (S\circ T)(v) = R((S\circ T)(v)) = R(S(T(v))).
    \end{align*}
\end{proof}

Let $A \in M_{m \times n}(\field)$ and $B \in M_{l \times m}(\field)$. Then, $L_A : \field^n \to \field^m$ and $L_B : \field^m \to \field^l$, and have composition $L_B \circ L_A : \field^n \to \field^l$. We know that $L_B \circ L_A$ is a linear transformation, and thus must be equal to $L_C$ for some matrix $C \in M_{l \times n}(\field)$. Indeed, $C$ is the matrix representation of the transformation $[L_B \circ L_A]$, as proven previously. 

Let $\beta = \{e_1, \dots, e_n\}$ for $\field^n$, then
\begin{align*}
    [L_B \circ L_A] = \begin{pmatrix}
        \vert &  &  \vert \\
        L_B \circ L_A(e_1) & \cdots & L_B\circ L_A(e_n)\\
        \vert &  & \vert
    \end{pmatrix} = \begin{pmatrix}
        \vert &  & \vert \\
        B\cdot (A \cdot e_1) & \cdots & B \cdot (A \cdot e_n)\\
        \vert & & \vert
    \end{pmatrix}
\end{align*}

\begin{definition}[Matrix Multiplication]
    For matrices $A \in M_{m \times n}(\field)$ and $B \in M_{l \times m}(\field)$, define their product $B \cdot A$ to be the matrix \begin{align*}
        [L_B \circ L_A] =
        \begin{pmatrix}
            \vert &  & \vert\\
            B\cdot (A \cdot e_1) & \cdots & B \cdot (A \cdot e_n)\\
            \vert & & \vert
        \end{pmatrix} = \begin{pmatrix}
            \vert & & \vert\\
            B \cdot A^{(1)} &\cdots & B \cdot A^{(2)}\\
            \vert & & \vert
        \end{pmatrix} = \left(c_{ij}\right)_{1 \leq i \leq l}^{1 \leq j \leq n}
    \end{align*}
    where $A^{(j)}$ is the $j$th column of $A$, $c_{ij} \defeq \begin{pmatrix}
        - & B_{(i)} & - 
    \end{pmatrix} \cdot \begin{pmatrix}
        \vert \\
        A^{(j)}\\
        \vert
    \end{pmatrix}$.
\end{definition}

\begin{proposition}
    $[L_B \circ L_A] = B \cdot A$, ie $L_B \circ L_A = L_{B \cdot A}$.
\end{proposition}
\begin{proof}
    Follows from our definition.
\end{proof}

\begin{corollary}
    Matrix multiplication is association; $C \cdot (B \cdot A) = (C \cdot B) \cdot A$ for $A \in M_{m \times n}(\field), B \in M_{l \times m}(\field), C \in M_{k \times l}(\field)$.
\end{corollary}
\begin{proof}
    $C\cdot (B \cdot A) = [L_C \circ (L_B \circ L_A)] = [(L_C\circ L_B) \circ L_A] = (C \cdot B) \cdot A$.
\end{proof}

\begin{remark}
    This is proven by the linear transformation representation of matrices; try proving this \emph{directly} from our definition.
\end{remark}

\begin{corollary}
    Let $V, W, U$ be finite-dimensional vector spaces over $\field$, $T : V \to W, S : W \to U$ be linear transformations and $\alpha, \beta, \gamma$ be bases for $V, W, U$ resp. Then, \[
    [S \circ T]_\alpha^\gamma = [S]_\beta^\gamma \cdot [T]_\alpha^\beta.    
    \]
\end{corollary}
\begin{proof}
    Follows from the commutativity of the diagrams:
\[
 % https://q.uiver.app/#q=WzAsNixbMCwwLCJWIl0sWzEsMCwiVyJdLFsyLDAsIlUiXSxbMCwxLCJcXG1hdGhiYntGfV5uIl0sWzEsMSwiXFxtYXRoYmJ7Rn1ebSJdLFsyLDEsIlxcbWF0aGJie0Z9XmwiXSxbMCwxLCJUIl0sWzEsMiwiUyJdLFsxLDQsIlxcc2ltIiwyXSxbMiw1LCJcXHNpbSIsMl0sWzMsNCwiW1RdX1xcYWxwaGFeXFxiZXRhIiwyXSxbNCw1LCJbU11fXFxiZXRhXlxcZ2FtbWEiLDJdLFswLDMsIlxcc2ltIiwyXV0=    
\begin{tikzcd}
        V & W & U \\
        {\mathbb{F}^n} & {\mathbb{F}^m} & {\mathbb{F}^l}
        \arrow["T", from=1-1, to=1-2]
        \arrow["S", from=1-2, to=1-3]
        \arrow["\wr"', from=1-2, to=2-2]
        \arrow["\wr"', from=1-3, to=2-3]
        \arrow["{[T]_\alpha^\beta}"', from=2-1, to=2-2]
        \arrow["{[S]_\beta^\gamma}"', from=2-2, to=2-3]
        \arrow["\wr"', from=1-1, to=2-1]
    \end{tikzcd}
    \qquad \iff\qquad 
    % https://q.uiver.app/#q=WzAsNCxbMCwwLCJWIl0sWzEsMCwiVSJdLFswLDEsIlxcbWF0aGJie0Z9Xm4iXSxbMSwxLCJcXG1hdGhiYntGfV5sIl0sWzAsMiwiXFxzaW0iLDJdLFsxLDMsIlxcc2ltIiwyXSxbMCwxLCJUIFxcY2lyYyBTIl0sWzIsMywiW1MgXFxjaXJjIFRdX1xcYWxwaGFeXFxnYW1tYSIsMl1d
    \begin{tikzcd}
        V & U \\
        {\mathbb{F}^n} & {\mathbb{F}^l}
        \arrow["\wr"', from=1-1, to=2-1]
        \arrow["\wr"', from=1-2, to=2-2]
        \arrow["{T \circ S}", from=1-1, to=1-2]
        \arrow["{[S \circ T]_\alpha^\gamma}"', from=2-1, to=2-2]
    \end{tikzcd}
\]    
    In "words", for $v \in V$,
    \begin{align*}
        [S \circ T]_\alpha^\gamma \cdot [v]_\alpha = [(S \circ T)(v)]_\alpha^\gamma = [S(T(v))]_\alpha = [S]_\beta^\gamma \cdot [T(v)]_\beta = [S]_\beta^\gamma \cdot [T]_\alpha^\beta \cdot [v]_\alpha,
    \end{align*}
    ie we have shown that $L_{[S \circ T]_\alpha^\gamma} = L_{[S]_\beta^\gamma \cdot [T]_\alpha^\beta}$. Because $A \mapsto L_A$ is an isomorphism, it follows that $[S \circ T]_\alpha^\gamma = [S]_\beta^\gamma \cdot [T]_\alpha^\beta$.
\end{proof}